theories/interpreter_func.v
@@ -76,14 +76,14 @@ Inductive res_step'
     (~ fragment_typeable s f [::] es) ->
     res_step' hs s f es
 | RS'_break k bvs :
-    (exists i j lh,
+    (exists i j (lh: lholed i),
       i + k = j /\
-      lfilledInd i lh (vs_to_es bvs ++ [::AI_basic (BI_br j)]) es /\
+      lfill lh (vs_to_es bvs ++ [::AI_basic (BI_br j)]) = es /\
       empty_vs_base lh) ->
     res_step' hs s f es
 | RS'_return rvs :
-    (exists i lh,
-      lfilledInd i lh (vs_to_es rvs ++ [:: AI_basic BI_return]) es /\
+    (exists i (lh: lholed i),
+      lfill lh (vs_to_es rvs ++ [:: AI_basic BI_return]) = es /\
       empty_vs_base lh) ->
     res_step' hs s f es
 | RS'_normal hs' s' f' es' :
@@ -98,18 +98,18 @@ Inductive res_step'_separate_e
     res_step'_separate_e hs s f ves e
 
 | RS''_break k bvs :
-    (exists i j lh,
+    (exists i j (lh: lholed i),
       i + k = j /\
-      lfilledInd i lh
-        (vs_to_es bvs ++ [:: AI_basic (BI_br j)]) (vs_to_es ves ++ [:: e]) /\
+      lfill lh
+        (vs_to_es bvs ++ [:: AI_basic (BI_br j)]) = (vs_to_es ves ++ [:: e]) /\
       empty_vs_base lh) ->
     res_step'_separate_e hs s f ves e
 
 | RS''_return rvs :
     (e = AI_basic BI_return /\ rvs = ves) \/
-    (exists ln les es i lh,
+    (exists ln les es i (lh: lholed i),
       e = AI_label ln les es /\
-      lfilledInd i lh (vs_to_es rvs ++ [:: AI_basic BI_return]) es /\
+      lfill lh (vs_to_es rvs ++ [:: AI_basic BI_return]) = es /\
       empty_vs_base lh) ->
     res_step'_separate_e hs s f ves e
 | RS''_normal hs' s' f' es' :
@@ -132,7 +132,7 @@ Definition config_one_tuple_without_e := (host_state * store_record * frame * li
 
 (* TODO auto instantiate lh, k? *)
 Ltac solve_lfilled :=
-  unfold lfilled, lfill, vs_to_es;
+  unfold lfill, vs_to_es;
   try rewrite v_to_e_is_const_list; apply/eqP; simplify_lists => //;
   repeat rewrite List.app_nil_r.
 
@@ -199,7 +199,7 @@ Ltac simpl_reduce_simple :=
       _ _ _ (vs_to_es (?vs ++ ?ves') ++ [:: ?e])
       _ _ _ (vs_to_es ?ves' ++ [:: ?e']) =>
         eapply r_label with
-          (k := 0) (lh := (LH_base (vs_to_es ves') [::]))
+          (k := 0) (lh := (LH_base (rev ves') [::]))
           (es := vs_to_es vs ++ [:: e])
           (es' := [:: e']);
         try solve_lfilled; apply r_simple
@@ -230,47 +230,46 @@ Qed.
 
 Lemma break_rec : forall e es es'' ves k bvs,
   split_vals_e es = (ves, e :: es'') ->
-  (exists i j lh,
+  (exists i j (lh: lholed i),
     i + k = j /\
-    lfilledInd i lh
-      (vs_to_es bvs ++ [:: AI_basic (BI_br j)]) (vs_to_es (rev ves) ++ [:: e]) /\
+    lfill lh
+      (vs_to_es bvs ++ [:: AI_basic (BI_br j)]) = (vs_to_es (rev ves) ++ [:: e]) /\
     empty_vs_base lh) ->
-  exists i j lh,
+  exists i j (lh: lholed i),
    i + k = j /\
-   lfilledInd i lh (vs_to_es bvs ++ [:: AI_basic (BI_br j)]) es /\
+   lfill lh (vs_to_es bvs ++ [:: AI_basic (BI_br j)]) = es /\
    empty_vs_base lh.
 Proof.
   intros e es es'' ves k bvs Hsplit
-    [i [j [[lh_vs lh_es | lh_vs n lh_es' lh' lh_es] [Heqj [Hlf Hbase]]]]];
+    [i [j [[lh_vs lh_es | k0 lh_vs n lh_es' lh' lh_es] [Heqj [Hlf Hbase]]]]];
     apply split_vals_e_v_to_e_duality in Hsplit; subst es; unfold vs_to_es.
   - destruct lh_vs => //.
-    inversion Hlf as [???? H1 H2 H3 Heqes|]; subst; clear Hlf.
+    simpl in Hlf.
+    rewrite -catA in Hlf.
+    unfold vs_to_es in Hlf.
+    apply ves_cat_e_split in Hlf as [Heq [<- ->]] => //; try by apply v_to_e_is_const_list.
     exists 0, k, (LH_base [::] es''). repeat split => //.
-    rewrite add0n -catA in Heqes. unfold vs_to_es in Heqes.
-    apply ves_cat_e_split in Heqes as [-> [<- ->]] => //;
+    rewrite /vs_to_es revK in Heq.
+    rewrite add0n in Heqj; subst j.
+    rewrite Heq.
+    by solve_lfilled.
+  - simpl in Hlf.
+    rewrite/vs_to_es revK in Hlf.
+    apply ves_cat_e_split in Hlf as [Heq [<- ->]] => //;
       try by apply v_to_e_is_const_list.
-    rewrite revK.
-    replace (AI_basic (BI_br k) :: es'')
-      with ([:: AI_basic (BI_br k)] ++ es'') => //.
-    by rewrite catA; apply LfilledBase.
-  - inversion Hlf as [ | i' vs0 m es'0 lh'0 es''0 es0 LI Hconst Hlf0 H1 H2 H5 Heqes].
-    subst i vs0 m es'0 lh'0 es''0 es0.
-    unfold vs_to_es in Heqes.
-    apply ves_cat_e_split in Heqes as [-> [<- ->]] => //;
-      try by apply v_to_e_is_const_list.
-    exists i'.+1, j, (LH_rec (v_to_e_list ves) n lh_es' lh' es'').
-    by repeat split => //; apply LfilledRec => //; apply v_to_e_is_const_list.
+    exists k0.+1, j, (LH_rec ves n lh_es' lh' es'').
+    by repeat split => //.
 Qed.
 
 Lemma return_rec : forall e es es'' ves rvs,
   split_vals_e es = (ves, e :: es'') ->
   (e = AI_basic BI_return /\ rvs = rev ves) \/
-  (exists ln les es i lh,
+  (exists ln les es i (lh: lholed i),
     e = AI_label ln les es /\
-    lfilledInd i lh (vs_to_es rvs ++ [:: AI_basic BI_return]) es /\
+    lfill lh (vs_to_es rvs ++ [:: AI_basic BI_return]) = es /\
     empty_vs_base lh) ->
-  exists i lh,
-  lfilledInd i lh (vs_to_es rvs ++ [:: AI_basic BI_return]) es /\
+  exists i (lh: lholed i),
+  lfill lh (vs_to_es rvs ++ [:: AI_basic BI_return]) = es /\
   empty_vs_base lh.
 Proof.
   intros e es es'' ves rvs Hsplit H.
@@ -279,11 +278,10 @@ Proof.
   - subst rvs. unfold vs_to_es. rewrite revK.
     exists 0, (LH_base [::] es'').
     split => //.
-    apply/lfilledP. solve_lfilled. by rewrite <- catA.
-  - exists (i.+1), (LH_rec (v_to_e_list ves) ln les lh es'').
+    by solve_lfilled.
+  - exists (i.+1), (LH_rec ves ln les lh es'').
     replace (AI_label ln les es :: es'') with ([:: AI_label ln les es] ++ es'') => //.
-    split => //.
-    by apply LfilledRec => //; apply v_to_e_is_const_list.
+    by split => //; subst.
 Qed.
 
 Lemma reduce_rec : forall (hs hs' : host_state) s s' f f' e es es' es'' ves res,
@@ -297,7 +295,7 @@ Proof.
   subst es es'.
   eapply r_label with (k := 0) (lh := (LH_base [::] es'')).
   - by apply Hreduce.
-  - solve_lfilled. by rewrite <- catA.
+  - by solve_lfilled. 
   - by solve_lfilled.
 Qed.
 
@@ -320,7 +318,7 @@ Proof.
   destruct e => //.
   apply split_vals_e_v_to_e_duality in Hsplit. subst es.
   move/orP in Hesves.
-  apply r_simple. eapply rs_trap with (lh := LH_base (vs_to_es (rev ves)) es'');
+  apply r_simple. eapply rs_trap with (lh := LH_base ves es'');
     try by solve_lfilled.
   destruct Hesves as [Hes | Hves].
   - assert (size es'' > 0); first by destruct es'' => //.
@@ -378,7 +376,7 @@ Lemma reduce_nop : forall (hs : host_state) s f ves,
 Proof.
   intros ??? ves.
   eapply r_label with
-    (k := 0) (lh := (LH_base (vs_to_es ves) [::]))
+    (k := 0) (lh := (LH_base (rev ves) [::]))
     (es := [:: AI_basic BI_nop])
     (es' := [::]); try by solve_lfilled.
   apply r_simple. by apply rs_nop.
@@ -391,7 +389,7 @@ Lemma reduce_drop : forall (hs : host_state) s f v ves',
 Proof.
   intros ??? v ves'.
   eapply r_label with
-    (k := 0) (lh := (LH_base (vs_to_es ves') [::]))
+    (k := 0) (lh := (LH_base (rev ves') [::]))
     (es := vs_to_es [:: v] ++ [:: AI_basic BI_drop])
     (es' := [::]); try by solve_lfilled.
   apply r_simple. by apply rs_drop.
@@ -476,7 +474,7 @@ Proof.
   injection Hsplit as Heqves' Heqves''.
   replace ves with (ves' ++ ves''); last by subst ves' ves''; rewrite cat_take_drop.
   eapply r_label with
-    (k := 0) (lh := (LH_base (vs_to_es ves'') [::])).
+    (k := 0) (lh := (LH_base (rev ves'') [::])).
   apply r_simple.
   eapply rs_block
     with (vs := vs_to_es ves') (t1s := t1s) => //.
@@ -489,7 +487,7 @@ Proof.
     (* TODO put symmetry into the ltac? *)
     by symmetry; if_lias.
   - by solve_lfilled.
-  - solve_lfilled. apply List.app_inj_tail_iff. by split; subst m.
+  - subst; by solve_lfilled.
 Qed.
 
 Lemma block_error : forall s f ves bt1s bt2s es,
@@ -522,7 +520,7 @@ Proof.
     by symmetry; if_lias.
   }
   eapply r_label with
-    (k := 0) (lh := (LH_base (vs_to_es ves'') [::])).
+    (k := 0) (lh := (LH_base (rev ves'') [::])).
   - apply r_simple.
     eapply rs_loop with (vs := vs_to_es ves') (t1s := t1s) (t2s := t2s) (es := es) => //.
     * by apply v_to_e_is_const_list.
@@ -561,7 +559,7 @@ Lemma reduce_if_false : forall (hs : host_state) s f c ves ves' tf es1 es2,
 Proof.
   intros hs s f c ves ves' tf es1 es2 ? Heqc. subst ves.
   eapply r_label with
-    (k := 0) (lh := (LH_base (vs_to_es ves') [::])).
+    (k := 0) (lh := (LH_base (rev ves') [::])).
   - apply r_simple. by apply rs_if_false.
   - solve_lfilled.
     replace c with (Wasm_int.int_zero i32m) => //.
@@ -578,7 +576,7 @@ Lemma reduce_if_true : forall (hs : host_state) s f c ves ves' tf es1 es2,
 Proof.
   intros hs s f c ves ves' tf es1 es2 ? Heqc. subst ves.
   eapply r_label with
-    (k := 0) (lh := (LH_base (vs_to_es ves') [::]));
+    (k := 0) (lh := (LH_base (rev ves') [::]));
     try by solve_lfilled.
   apply r_simple. apply rs_if_true with (n := c).
   apply/eqP. by lias.
@@ -608,11 +606,11 @@ Proof.
 Qed.
 
 Lemma break_br : forall j ves,
-  exists (i j' : nat) (lh : lholed),
+  exists (i j' : nat) (lh : lholed i),
     i + j = j' /\
-    lfilledInd i lh
+    lfill lh
       (vs_to_es ves ++ [:: AI_basic (BI_br j')])
-      (vs_to_es ves ++ [:: AI_basic (BI_br j)]) /\
+      = (vs_to_es ves ++ [:: AI_basic (BI_br j)]) /\
     empty_vs_base lh.
 Proof.
   intros j ves.
@@ -621,7 +619,7 @@ Proof.
   replace (vs_to_es ves ++ [:: AI_basic (BI_br j)])
     with ([::] ++ (vs_to_es ves ++ [:: AI_basic (BI_br j)]) ++ [::]) at 2;
     last by rewrite <- catA.
-  by apply LfilledBase => //.
+  by solve_lfilled.
 Qed.
 
 Lemma reduce_br_if_true : forall (hs : host_state) s f c ves' j,
@@ -632,7 +630,7 @@ Lemma reduce_br_if_true : forall (hs : host_state) s f c ves' j,
 Proof.
   intros ??? c ves' j ?.
   apply r_label with
-    (k := 0) (lh := (LH_base (vs_to_es ves') [::]))
+    (k := 0) (lh := (LH_base (rev ves') [::]))
     (es := vs_to_es [::VAL_int32 c] ++ [:: AI_basic (BI_br_if j)])
     (es' := [:: AI_basic (BI_br j)]);
     try by solve_lfilled.
@@ -648,7 +646,7 @@ Proof.
   intros ??? c ves' j ?.
   (* TODO make simpl_reduce_simple applicable? *)
   eapply r_label with
-    (k := 0) (lh := (LH_base (vs_to_es ves') [::]))
+    (k := 0) (lh := (LH_base (rev ves') [::]))
     (es := vs_to_es [::VAL_int32 c] ++ [:: AI_basic (BI_br_if j)])
     (es' := [::]);
     try by solve_lfilled.
@@ -688,7 +686,7 @@ Lemma reduce_br_table : forall (hs : host_state) s f c ves' k j js js_at_k,
 Proof.
   intros ??? c ves' k j js js_at_k ???. subst k.
   eapply r_label with
-    (k := 0) (lh := (LH_base (vs_to_es ves') [::]));
+    (k := 0) (lh := (LH_base (rev ves') [::]));
     try by by solve_lfilled.
   apply r_simple. by apply rs_br_table.
 Qed.
@@ -702,7 +700,7 @@ Lemma reduce_br_table_length : forall (hs : host_state) s f c ves' k j js,
 Proof.
   intros ??? c ves' k j js ??. subst k.
   eapply r_label with
-    (k := 0) (lh := (LH_base (vs_to_es ves') [::]));
+    (k := 0) (lh := (LH_base (rev ves') [::]));
     try by solve_lfilled.
   apply r_simple. by apply rs_br_table_length.
 Qed.
@@ -752,7 +750,7 @@ Lemma reduce_call : forall (hs : host_state) s f ves j a,
     hs s f (vs_to_es ves ++ [:: AI_invoke a]).
 Proof.
   intros hs s f ves j a ?.
-  eapply r_label with (k := 0) (lh := (LH_base (vs_to_es ves) [::]));
+  eapply r_label with (k := 0) (lh := (LH_base (rev ves) [::]));
     try by solve_lfilled.
   apply r_call with (a := a) (i := j) => //.
 Qed.
@@ -779,7 +777,7 @@ Lemma reduce_call_indirect_success : forall (hs : host_state) s f c ves ves' j a
     hs s f (vs_to_es ves' ++ [:: AI_invoke a]).
 Proof.
   intros hs s f c ves ves' j a cl ????. subst ves.
-  eapply r_label with (k := 0) (lh := (LH_base (vs_to_es ves') [::]));
+  eapply r_label with (k := 0) (lh := (LH_base (rev ves') [::]));
     try by solve_lfilled.
   apply r_call_indirect_success with (cl := cl) => //.
   by apply/eqP.
@@ -795,7 +793,7 @@ Lemma reduce_call_indirect_failure_1 : forall (hs : host_state) s f c ves ves' j
     hs s f (vs_to_es ves' ++ [:: AI_trap]).
 Proof.
   intros hs s f c ves ves' j a cl ????. subst ves.
-  eapply r_label with (k := 0) (lh := (LH_base (vs_to_es ves') [::]));
+  eapply r_label with (k := 0) (lh := (LH_base (rev ves') [::]));
     try by solve_lfilled.
   eapply r_call_indirect_failure1 with (cl := cl) (a := a) => //.
   by apply/eqP; lias.
@@ -809,7 +807,7 @@ Lemma reduce_call_indirect_failure_2 : forall (hs : host_state) s f c ves ves' j
     hs s f (vs_to_es ves' ++ [:: AI_trap]).
 Proof.
   intros hs s f c ves ves' j ??. subst ves.
-  eapply r_label with (k := 0) (lh := (LH_base (vs_to_es ves') [::]));
+  eapply r_label with (k := 0) (lh := (LH_base (rev ves') [::]));
     try by solve_lfilled.
   by apply r_call_indirect_failure2.
 Qed.
@@ -856,7 +854,7 @@ Lemma reduce_get_local : forall (hs : host_state) s f ves j vs_at_j,
     hs s f (vs_to_es (vs_at_j :: ves)).
 Proof.
   intros hs s f ves j vs_at_j ??.
-  eapply r_label with (k := 0) (lh := (LH_base (vs_to_es ves) [::])).
+  eapply r_label with (k := 0) (lh := (LH_base (rev ves) [::])).
   - apply r_get_local with (j := j) (v := vs_at_j) => //.
   - by solve_lfilled.
   - by solve_lfilled.
@@ -894,7 +892,7 @@ Lemma reduce_set_local : forall (hs : host_state) s f f' v ves ves' j,
     hs s f' (vs_to_es ves').
 Proof.
   intros hs s f f' v ves ves' j ???. subst ves f'.
-  eapply r_label with (k := 0) (lh := (LH_base (vs_to_es ves') [::])).
+  eapply r_label with (k := 0) (lh := (LH_base (rev ves') [::])).
   - apply r_set_local with (i := j) (v := v) (vd := v) => //.
   - by solve_lfilled.
   - by solve_lfilled.
@@ -931,7 +929,7 @@ Lemma reduce_tee_local : forall (hs : host_state) s f v ves ves' j,
 Proof.
   intros hs s f v ves ves' j ?.
   subst ves.
-  eapply r_label with (k := 0) (lh := (LH_base (vs_to_es ves') [::])).
+  eapply r_label with (k := 0) (lh := (LH_base (rev ves') [::])).
   - apply r_simple.
     by apply rs_tee_local with (i := j) (v := AI_basic (BI_const v)).
   - by solve_lfilled.
@@ -955,7 +953,7 @@ Lemma reduce_get_global : forall (hs : host_state) s f ves j xx,
     hs s f (vs_to_es (xx :: ves)).
 Proof.
   intros hs s f ves j xx Heqxx.
-  eapply r_label with (k := 0) (lh := (LH_base (vs_to_es ves) [::])).
+  eapply r_label with (k := 0) (lh := (LH_base (rev ves) [::])).
   - by apply r_get_global with (i := j) (v := xx).
   - by solve_lfilled.
   - by solve_lfilled.
@@ -984,7 +982,7 @@ Lemma reduce_set_global : forall (hs : host_state) s s' f v ves ves' j,
     hs s' f (vs_to_es ves').
 Proof.
   intros hs s s' f v ves ves' j Heqs' ?. subst ves.
-  eapply r_label with (k := 0) (lh := (LH_base (vs_to_es ves') [::])).
+  eapply r_label with (k := 0) (lh := (LH_base (rev ves') [::])).
   - by apply r_set_global with (i := j) (v := v).
   - by solve_lfilled.
   - by solve_lfilled.
@@ -1029,7 +1027,7 @@ Lemma reduce_load_packed_success : forall (hs : host_state) s f c ves ves' t tp 
 Proof.
   intros hs s f c ves ves' t tp sx a off j mem_s_j bs ????. subst ves.
   (* XXX make this into an ltac? (selecting the LH_base) *)
-  eapply r_label with (k := 0) (lh := (LH_base (vs_to_es ves') [::]));
+  eapply r_label with (k := 0) (lh := (LH_base (rev ves') [::]));
     try by solve_lfilled.
   by apply r_load_packed_success with (i := j) (m := mem_s_j).
 Qed.
@@ -1044,7 +1042,7 @@ Lemma reduce_load_packed_failure : forall (hs : host_state) s f c ves ves' t tp 
     hs s f (vs_to_es ves' ++ [:: AI_trap]).
 Proof.
   intros hs s f c ves ves' t tp sx a off j mem_s_j ????. subst ves.
-  eapply r_label with (k := 0) (lh := (LH_base (vs_to_es ves') [::]));
+  eapply r_label with (k := 0) (lh := (LH_base (rev ves') [::]));
     try by solve_lfilled.
   by apply r_load_packed_failure with (i := j) (m := mem_s_j).
 Qed.
@@ -1059,7 +1057,7 @@ Lemma reduce_load_success : forall (hs : host_state) s f c ves ves' t a off j me
     hs s f (vs_to_es (wasm_deserialise bs t :: ves')).
 Proof.
   intros hs s f c ves ves' t a off j mem_s_j bs ????. subst ves.
-  eapply r_label with (k := 0) (lh := (LH_base (vs_to_es ves') [::]));
+  eapply r_label with (k := 0) (lh := (LH_base (rev ves') [::]));
     try by solve_lfilled.
   by apply r_load_success
     with (i := j) (m := mem_s_j) (bs := bs) (k := c) (off := off) (t := t).
@@ -1075,7 +1073,7 @@ Lemma reduce_load_failure : forall (hs : host_state) s f c ves ves' t a off j me
     hs s f (vs_to_es ves' ++ [:: AI_trap]).
 Proof.
   intros hs s f c ves ves' t a off j mem_s_j ????. subst ves.
-  eapply r_label with (k := 0) (lh := (LH_base (vs_to_es ves') [::]));
+  eapply r_label with (k := 0) (lh := (LH_base (rev ves') [::]));
     try by solve_lfilled.
   by apply r_load_failure with (i := j) (m := mem_s_j).
 Qed.
@@ -1141,7 +1139,7 @@ Lemma reduce_store_packed_success : forall (hs : host_state) s f c v ves ves' t 
     hs (upd_s_mem s (set_nth mem' s.(s_mems) j mem')) f (vs_to_es ves').
 Proof.
   intros hs s f c v ves ves' t tp a off j mem_s_j mem' ?????. subst ves.
-  eapply r_label with (k := 0) (lh := (LH_base (vs_to_es ves') [::])).
+  eapply r_label with (k := 0) (lh := (LH_base (rev ves') [::])).
   - by apply r_store_packed_success
       with (m := mem_s_j) (k := c) (off := off) (t := t) (v := v) (tp := tp).
   - by solve_lfilled.
@@ -1159,7 +1157,7 @@ Lemma reduce_store_packed_failure : forall (hs : host_state) s f c v ves ves' t 
     hs s f (vs_to_es ves' ++ [:: AI_trap]).
 Proof.
   intros hs s f c v ves ves' t tp a off j mem_s_j ?????. subst ves.
-  eapply r_label with (k := 0) (lh := (LH_base (vs_to_es ves') [::]));
+  eapply r_label with (k := 0) (lh := (LH_base (rev ves') [::]));
     try by solve_lfilled.
   by apply r_store_packed_failure with (i := j) (m := mem_s_j).
 Qed.
@@ -1175,7 +1173,7 @@ Lemma reduce_store_success : forall (hs : host_state) s f c v ves ves' t a off j
     hs (upd_s_mem s (set_nth mem' s.(s_mems) j mem')) f (vs_to_es ves').
 Proof.
   intros hs s f c v ves ves' t a off j mem_s_j mem' ?????. subst ves.
-  eapply r_label with (k := 0) (lh := (LH_base (vs_to_es ves') [::])).
+  eapply r_label with (k := 0) (lh := (LH_base (rev ves') [::])).
   - by apply r_store_success
       with (m := mem_s_j) (k := c) (off := off) (t := t) (v := v).
   - by solve_lfilled.
@@ -1193,7 +1191,7 @@ Lemma reduce_store_failure : forall (hs : host_state) s f c v ves ves' t a off j
     hs s f (vs_to_es ves' ++ [:: AI_trap]).
 Proof.
   intros hs s f c v ves ves' t a off j mem_s_j ?????. subst ves.
-  eapply r_label with (k := 0) (lh := (LH_base (vs_to_es ves') [::]));
+  eapply r_label with (k := 0) (lh := (LH_base (rev ves') [::]));
     try by solve_lfilled.
   by apply r_store_failure
     with (i := j) (m := mem_s_j) (k := c) (off := off) (t := t) (v := v).
@@ -1279,7 +1277,7 @@ Lemma reduce_current_memory : forall (hs : host_state) s f v ves s_mem_s_j j,
     hs s f (vs_to_es (v :: ves)).
 Proof.
   intros hs s f v ves s_mem_s_j j ???. subst v.
-  eapply r_label with (k := 0) (lh := (LH_base (vs_to_es ves) [::]));
+  eapply r_label with (k := 0) (lh := (LH_base (rev ves) [::]));
     try by solve_lfilled.
   (* TODO rename s_mem_s_j to m? *)
   by apply r_current_memory with (i := j) (m := s_mem_s_j).
@@ -1324,7 +1322,7 @@ Lemma reduce_grow_memory : forall (hs : host_state) s s' f c v ves' mem'' s_mem_
     hs s' f (vs_to_es (v :: ves')).
 Proof.
   intros hs s s' f c v ves' mem'' s_mem_s_j j l ??????. subst s' v l.
-  eapply r_label with (k := 0) (lh := (LH_base (vs_to_es ves') [::]));
+  eapply r_label with (k := 0) (lh := (LH_base (rev ves') [::]));
     try by solve_lfilled.
   by apply r_grow_memory_success with (m := s_mem_s_j) (c := c).
 Qed.
@@ -1339,7 +1337,7 @@ Lemma reduce_grow_memory_failure : forall (hs : host_state) s f c ves' s_mem_s_j
     hs s f (vs_to_es (VAL_int32 int32_minus_one :: ves')).
 Proof.
   intros hs s f c ves' s_mem_s_j j l ????. subst l.
-  eapply r_label with (k := 0) (lh := (LH_base (vs_to_es ves') [::]));
+  eapply r_label with (k := 0) (lh := (LH_base (rev ves') [::]));
     try by solve_lfilled.
   by eapply r_grow_memory_failure with (m := s_mem_s_j) (i := j).
 Qed.
@@ -1612,7 +1610,7 @@ Proof.
   replace ves with (ves' ++ ves''); last by subst ves' ves''; rewrite cat_take_drop.
   replace (vs_to_es (ves' ++ ves'')) with (vs_to_es ves'' ++ vs_to_es ves');
     last by unfold vs_to_es; rewrite rev_cat; rewrite v_to_e_cat.
-  eapply r_label with (k := 0) (lh := LH_base (vs_to_es ves'') [::]);
+  eapply r_label with (k := 0) (lh := LH_base (rev ves'') [::]);
     try by solve_lfilled.
   eapply r_invoke_native with (t1s := t1s) => //; try by assumption.
   (* TODO lias to apply length_is_size aggresively? *)
@@ -1641,7 +1639,7 @@ Proof.
   replace ves with (ves' ++ ves''); last by subst ves' ves''; rewrite cat_take_drop.
   replace (vs_to_es (ves' ++ ves'')) with (vs_to_es ves'' ++ vs_to_es ves');
     last by unfold vs_to_es; rewrite rev_cat; rewrite v_to_e_cat.
-  eapply r_label with (k := 0) (lh := LH_base (vs_to_es ves'') [::]);
+  eapply r_label with (k := 0) (lh := LH_base (rev ves'') [::]);
     try by solve_lfilled.
   eapply r_invoke_host_success with (t1s := t1s) (t2s := t2s) (h := cl') => //;
     try by assumption.
@@ -1671,7 +1669,7 @@ Proof.
   replace ves with (ves' ++ ves''); last by subst ves' ves''; rewrite cat_take_drop.
   replace (vs_to_es (ves' ++ ves'')) with (vs_to_es ves'' ++ vs_to_es ves');
     last by unfold vs_to_es; rewrite rev_cat; rewrite v_to_e_cat.
-  eapply r_label with (k := 0) (lh := LH_base (vs_to_es ves'') [::]);
+  eapply r_label with (k := 0) (lh := LH_base (rev ves'') [::]);
     try by solve_lfilled.
   eapply r_invoke_host_diverge with (t1s := t1s) (t2s := t2s) (h := cl') => //;
     try by assumption.
@@ -1744,7 +1742,7 @@ Lemma reduce_label_const : forall (hs : host_state) s f ves ln les es,
     hs s f (vs_to_es ves ++ es).
 Proof.
   intros hs s f ves ln les es Htrap.
-  eapply r_label with (k := 0) (lh := LH_base (vs_to_es ves) [::]);
+  eapply r_label with (k := 0) (lh := LH_base (rev ves) [::]);
     try by solve_lfilled.
   by apply r_simple; apply rs_label_const.
 Qed.
@@ -1780,36 +1778,16 @@ Lemma reduce_label_rec : forall (hs hs' : host_state) s s' f f' es es' ves ln le
 Proof.
   intros hs hs' s s' f f' es es' ves ln les IH.
   eapply r_label with
-    (k := 1) (lh := (LH_rec (vs_to_es ves) ln les (LH_base [::] [::]) [::]));
+    (k := 1) (lh := (LH_rec (rev ves) ln les (LH_base [::] [::]) [::]));
     try by solve_lfilled.
   by apply IH.
 Qed.
 
-Lemma lfilled_take_v_to_e : forall i lh n ves e es,
-  n <= size ves ->
-  lfilledInd i lh (vs_to_es ves ++ [:: e]) es ->
-  exists lh', lfilledInd i lh' (vs_to_es (take n ves) ++ [:: e]) es.
-Proof.
-  intros i lh n ves e es Hn H.
-  unfold vs_to_es. unfold vs_to_es in H.
-  remember (size ves - n) as n'.
-  assert (Hn' : n = (size ves - n')). { by lias. }
-  rewrite Hn'.
-  rewrite <- drop_rev. rewrite v_to_e_drop.
-  apply lfilled_collapse1 with (l := n) in H as [lh' H].
-  - exists lh'.
-    rewrite length_is_size in H. rewrite v_to_e_size in H. rewrite size_rev in H.
-    subst n'. by apply H.
-  - by apply v_to_e_is_const_list.
-  - rewrite length_is_size. rewrite v_to_e_size. rewrite size_rev.
-    by lias.
-Qed.
-
 Lemma reduce_label_break_rec : forall (hs : host_state) s f ln les es ves bvs,
   ln <= length bvs ->
-  (exists i j lh,
+  (exists i j (lh: lholed i),
     i + 0 = j /\
-    lfilledInd i lh (vs_to_es bvs ++ [:: AI_basic (BI_br j)]) es /\
+    lfill lh (vs_to_es bvs ++ [:: AI_basic (BI_br j)]) = es /\
     empty_vs_base lh) ->
   reduce
     hs s f (vs_to_es ves ++ [:: AI_label ln les es])
@@ -1817,34 +1795,33 @@ Lemma reduce_label_break_rec : forall (hs : host_state) s f ln les es ves bvs,
 Proof.
   intros hs s f ln les es ves bvs Hlen [i [j [lh [Heqj [HLF Hbase]]]]].
   rewrite addn0 in Heqj. subst j.
-  apply lfilled_take_v_to_e with (n := ln) in HLF as [lh' HLF] => //.
-  move/lfilledP in HLF.
+  unfold vs_to_es in HLF.
+  erewrite lfill_push_base_vs' in HLF; last (by rewrite length_is_size v_to_e_size size_rev; rewrite length_is_size in Hlen; apply Hlen); eauto.
   unfold vs_to_es. rewrite rev_cat. rewrite <- v_to_e_cat.
-  eapply r_label with (k := 0) (lh := LH_base (vs_to_es ves) [::]);
+  eapply r_label with (k := 0) (lh := LH_base (rev ves) [::]);
     try by solve_lfilled.
-  apply r_simple. apply rs_br with (i := i) (lh := lh') => //.
-  - by apply v_to_e_is_const_list.
-  - rewrite length_is_size. rewrite length_is_size in Hlen.
-    rewrite v_to_e_size. rewrite size_rev. rewrite size_take.
-    by if_lias.
+  subst es.
+  apply r_simple. eapply rs_br; first by apply v_to_e_is_const_list.
+  - rewrite length_is_size v_to_e_size size_rev size_takel => //; rewrite length_is_size in Hlen.
+  - do 2 (erewrite lfill_push_base_vs; eauto).
+    by rewrite length_is_size v_to_e_size size_rev rev_take v_to_e_drop.
 Qed.
 
 Lemma label_break_rec : forall n ln les es bvs ves,
-  (exists i j lh,
+  (exists i j (lh: lholed i),
     i + n.+1 = j /\
-    lfilledInd i lh (vs_to_es bvs ++ [:: AI_basic (BI_br j)]) es /\
+    lfill lh (vs_to_es bvs ++ [:: AI_basic (BI_br j)]) = es /\
     empty_vs_base lh) ->
-  (exists i j lh,
+  (exists i j (lh: lholed i),
     i + n = j /\
-    lfilledInd i lh
+    lfill lh
       (vs_to_es bvs ++ [:: AI_basic (BI_br j)])
-      (vs_to_es ves ++ [:: AI_label ln les es]) /\
+      = (vs_to_es ves ++ [:: AI_label ln les es]) /\
     empty_vs_base lh).
 Proof.
-  intros n ln les es bvs ves [i [j [lh [Heqj [HLF Hbase]]]]].
-  exists (i.+1), j, (LH_rec (vs_to_es ves) ln les lh [::]).
-  repeat split; try by lias.
-  by apply LfilledRec => //; apply v_to_e_is_const_list.
+  intros n ln les es bvs ves [i [j [lh [Heqj [<- Hbase]]]]].
+  exists (i.+1), j, (LH_rec (rev ves) ln les lh [::]).
+  repeat split => /=; by lias.
 Qed.
 
 Lemma br_arguments_length: forall s C ts t_br j bvs,
@@ -1874,41 +1851,42 @@ Proof.
   repeat rewrite length_is_size; by lias.
 Qed.
 
-Lemma lfilled_hole_typed_br : forall lh s C es ts i m j bvs,
+Lemma lfilled_hole_typed_br : forall i (lh: lholed i) s C es ts m j bvs,
   e_typing s C es (Tf [::] ts) ->
   empty_vs_base lh ->
-  lfilledInd i lh (v_to_e_list bvs ++ [:: AI_basic (BI_br j)]) es ->
+  lfill lh (v_to_e_list bvs ++ [:: AI_basic (BI_br j)]) = es ->
   i + m = j ->
   exists ts C',
     List.nth_error C'.(tc_label) j = List.nth_error C.(tc_label) m /\
     e_typing s C' (v_to_e_list bvs ++ [:: AI_basic (BI_br j)]) (Tf [::] ts).
 Proof.
-  induction lh as [vs es' | vs k es' lh' IH]; move => s C es ts i m j bvs Hetype Hbase Hlf Hj.
+  move => i.
+  induction lh as [vs es' | ? vs k es' lh' IH]; move => s C es ts m j bvs Hetype Hbase Hlf Hj => /=; subst.
   - destruct vs => //.
-    inversion Hlf; subst; simpl in Hetype; clear Hlf.
+    simpl in Hetype.
     apply e_composition_typing in Hetype
-      as [? [t0s [ts' [t1s' [Ht0s [Hts'' [Hetypebvs Hetype]]]]]]].
-    apply_cat0_inv Ht0s. simpl in Hts''; subst.
+      as [? [t0s [ts' [t1s' [Heq [-> [Hetypebvs Hetype]]]]]]].
+    apply_cat0_inv Heq => /=.
     by exists t1s', C.
-  - inversion Hlf as [ | i' vs0 n es'0 lh'0 es''0 es0 LI Hconst Hlf0].
-    subst i es vs0 n es'0 lh'0 es''0 es0; clear Hlf.
+  - simpl in *.
     apply e_composition_typing in Hetype
-      as [? [t0s [ts' [t1s' [Ht0s [Hts'' [Hetypevs Hetype]]]]]]].
-    apply_cat0_inv Ht0s; subst ts.
+      as [? [t0s [ts' [t1s' [Ht0s [-> [Hetypevs Hetype]]]]]]].
+    apply_cat0_inv Ht0s.
+    rewrite - cat1s in Hetype.
     apply e_composition_typing in Hetype
-      as [? [t0s' [ts'' [t1s'' [Ht0s [Hts'' [Hetypebvs Hetype]]]]]]].
+      as [? [t0s' [ts'' [t1s'' [-> [-> [Hetypebvs Hetype]]]]]]].
     apply Label_typing in Hetypebvs
       as [? [t2s' [-> [Hetypees' [HetypeLI Hlen]]]]].
 
-    apply IH with (bvs := bvs) (i := i') (m := m.+1) (j := j) in HetypeLI
+    eapply IH with (bvs := bvs) (m := m.+1) in HetypeLI
       as [ts''' [C' [Hlab Hetypebase]]] => //; last by lias.
-    exists ts''', C' => //.
+    by exists ts''', C' => //.
 Qed.
 
-Lemma lfilled_br_empty_vs_base : forall lh s C ln les es t1s t2s i bvs,
+Lemma lfilled_br_empty_vs_base : forall i (lh: lholed i) s C ln les es t1s t2s bvs,
   e_typing s C [:: AI_label ln les es] (Tf t1s t2s) ->
   empty_vs_base lh ->
-  lfilledInd i lh (vs_to_es bvs ++ [:: AI_basic (BI_br i)]) es ->
+  lfill lh (vs_to_es bvs ++ [:: AI_basic (BI_br i)]) = es ->
   length bvs >= ln.
 Proof.
   move => lh s C ln les es t1s t2s i bvs Hetype Hbase Hlf.
@@ -1921,9 +1899,9 @@ Proof.
 Qed.
 
 Lemma label_error_break_rec : forall s f ves bvs ln les es,
-  (exists i j lh,
+  (exists i j (lh: lholed i),
     i + 0 = j /\
-    lfilledInd i lh (vs_to_es bvs ++ [:: AI_basic (BI_br j)]) es /\
+    lfill lh (vs_to_es bvs ++ [:: AI_basic (BI_br j)]) = es /\
     empty_vs_base lh) ->
   (ln <= length bvs) = false ->
   ~ fragment_typeable s f ves [:: AI_label ln les es].
@@ -1958,7 +1936,7 @@ Lemma reduce_local_const : forall (hs : host_state) s f ves ln lf es,
     hs s f (vs_to_es ves ++ es).
 Proof.
   intros hs s f ves ln lf es ??.
-  eapply r_label with (k := 0) (lh := LH_base (vs_to_es ves) [::]);
+  eapply r_label with (k := 0) (lh := LH_base (rev ves) [::]);
     try by solve_lfilled.
   apply r_simple. by apply rs_local_const => //; apply/eqP.
 Qed.
@@ -1977,17 +1955,6 @@ Proof.
   rewrite length_is_size size_map in Hlen'.
   rewrite length_is_size v_to_e_size in Hlen.
   by move/eqP in Hlen.
-Qed.
-
-Lemma lfilled_collapse': forall n lh vs es LI,
-    lfilledInd n lh (vs ++ es) LI ->
-    const_list vs ->
-    exists lh', lfilledInd n lh' es LI.
-Proof.
-  intros n lh vs es LI HLF Hconst.
-  apply lfilled_collapse1 with (l := 0) in HLF => //.
-  rewrite subn0 in HLF.
-  by rewrite drop_size in HLF => //.
 Qed.
 
 Lemma local_error_rec : forall s f es ves ln lf,
@@ -2011,45 +1978,42 @@ Proof.
   by apply Hetype.
 Qed.
 
-Lemma lfilled_labels : forall lh i j k s C bvs es t1s t2s,
+Lemma lfilled_labels : forall i (lh: lholed i) j k s C bvs es t1s t2s,
   size C.(tc_label) = k ->
   e_typing s C es (Tf t1s t2s) ->
-  lfilledInd i lh (vs_to_es bvs ++ [:: AI_basic (BI_br j)]) es ->
+  lfill lh (vs_to_es bvs ++ [:: AI_basic (BI_br j)]) = es ->
   j < i + k.
 Proof.
-  induction lh as [vs es' | vs m es' lh' IH];
-    intros i j k s C bvs es t1s t2s Hlab Hetype Hlf;
-    inversion Hlf as [ | i' vs0 m' es'0 lh'0 es''0 es0 LI Hconst Hlf0].
-  - subst. repeat rewrite catA in Hetype.
-    apply e_composition_typing in Hetype as [? [? [? [? [-> [-> [Hetype _]]]]]]].
+  move => i.
+  induction lh as [vs es' | k0 vs m es' lh' IH];
+    intros j k s C bvs es t1s t2s Hlab Hetype Hlf; subst; simpl in Hetype; repeat rewrite catA in Hetype.
+  - apply e_composition_typing in Hetype as [? [? [? [? [-> [-> [Hetype _]]]]]]].
     apply e_composition_typing in Hetype as [? [? [? [? [-> [-> [_ Hetypebr]]]]]]].
     apply et_to_bet in Hetypebr; last by auto_basic.
     by apply (Break_typing host_instance) in Hetypebr as [? [? [Hj [??]]]]; auto.
-  - subst i k vs0 m' es'0 lh'0 es''0 es0 es.
+  - rewrite - cat1s in Hetype.
     apply e_composition_typing in Hetype as [? [t0s [? [t1s' [-> [-> [_ Hetype]]]]]]].
     apply e_composition_typing in Hetype as [? [t1s [? [t2s' [-> [-> [Hetype _]]]]]]].
     apply Label_typing in Hetype as [ts [t3s' [-> [_ [HetypeLI Hlen]]]]].
-    eapply IH with (C := (upd_label C ([:: ts] ++ tc_label C))) in Hlf0 => //;
-      last by apply HetypeLI.
-    by simpl in Hlf0; lias.
+    eapply IH in HetypeLI => //.
+    simpl in *; by lias.
 Qed.
 
-Lemma lfilled_labels_emp : forall lh i s C bvs j es t1s t2s,
+Lemma lfilled_labels_emp : forall i (lh: lholed i) s C bvs j es t1s t2s,
   C.(tc_label) = [::] ->
   e_typing s C es (Tf t1s t2s) ->
-  lfilledInd i lh (vs_to_es bvs ++ [:: AI_basic (BI_br j)]) es ->
+  lfill lh (vs_to_es bvs ++ [:: AI_basic (BI_br j)]) = es ->
   j < i.
 Proof.
-  intros lh i s C bvs j es t1s t2s Hlab Hetype Hlf.
-  apply f_equal with (f := size) in Hlab; simpl in Hlab.
-  replace i with (i + 0); last by apply addn0.
-  by eapply lfilled_labels; eauto.
+  move => i lh s C bvs j es t1s t2s Hlab Hetype /= Hlf.
+  eapply lfilled_labels in Hlf => //; last by eauto.
+  by rewrite Hlab addn0 in Hlf.
 Qed.
 
 Lemma local_error_break_rec : forall s f es ves ln lf n bvs,
-  (exists i j lh,
+  (exists i j (lh: lholed i),
     i + n = j /\
-    lfilledInd i lh (vs_to_es bvs ++ [:: AI_basic (BI_br j)]) es /\
+    lfill lh (vs_to_es bvs ++ [:: AI_basic (BI_br j)]) = es /\
     empty_vs_base lh) ->
   ~ fragment_typeable s f ves [:: AI_local ln lf es].
 Proof.
@@ -2064,11 +2028,10 @@ Proof.
   by lias.
 Qed.
 
-(* XXX this could maybe be simplified by using lfilled_collapse1 more directly *)
 Lemma reduce_local_return_rec : forall (hs : host_state) s f lf rvs ves ln es,
   ln <= length rvs ->
-  (exists i lh,
-    lfilledInd i lh (vs_to_es rvs ++ [:: AI_basic BI_return]) es /\
+  (exists i (lh: lholed i),
+    lfill lh (vs_to_es rvs ++ [:: AI_basic BI_return]) = es /\
     empty_vs_base lh) ->
   reduce
     hs s f (vs_to_es ves ++ [:: AI_local ln lf es])
@@ -2076,46 +2039,40 @@ Lemma reduce_local_return_rec : forall (hs : host_state) s f lf rvs ves ln es,
 Proof.
   intros hs s f lf rvs ves ln es Hlen [i [lh [HLF _]]].
 
-  eapply r_label with (k := 0) (lh := LH_base (vs_to_es ves) [::]);
+  eapply r_label with (k := 0) (lh := LH_base (rev ves) [::]);
     try by solve_lfilled.
-  assert (length (v_to_e_list (rev (take ln rvs))) = ln).
-  {
-    rewrite length_is_size in Hlen. rewrite length_is_size.
-    rewrite v_to_e_size. rewrite size_rev. rewrite size_take. by if_lias.
-  }
 
-  apply lfilled_take_v_to_e with (n := ln) in HLF as [lh' HLF];
-    last by rewrite length_is_size in Hlen.
-
+  erewrite lfill_push_base_vs' in HLF; last (by rewrite length_is_size v_to_e_size size_rev; rewrite length_is_size in Hlen; apply Hlen); try by eauto.
   apply r_simple.
-  apply rs_return with (i := i) (lh := lh') => //;
-    first by apply v_to_e_is_const_list.
-
-  by apply/lfilledP.
+  eapply rs_return; eauto; [ by apply v_to_e_is_const_list | rewrite length_is_size v_to_e_size size_rev size_takel => //; rewrite length_is_size in Hlen | ].
+  subst es.
+  by rewrite length_is_size v_to_e_size size_rev rev_take v_to_e_drop.
 Qed.
 
-Lemma lfilled_hole_typed_return : forall lh s C es ts i rvs,
+Lemma lfilled_hole_typed_return : forall i (lh: lholed i) s C es ts rvs,
   e_typing s C es (Tf [::] ts) ->
   empty_vs_base lh ->
-  lfilledInd i lh (v_to_e_list rvs ++ [:: AI_basic BI_return]) es ->
+  lfill lh (v_to_e_list rvs ++ [:: AI_basic BI_return]) = es ->
   exists ts C',
     C'.(tc_return) = C.(tc_return) /\
     e_typing s C' (v_to_e_list rvs ++ [::AI_basic BI_return]) (Tf [::] ts).
 Proof.
-  induction lh as [vs es' | vs j es' lh' IH]; move => s C es ts i rvs Hetype Hbase Hlf.
+  move => i.
+  induction lh as [vs es' | ? vs j es' lh' IH]; move => s C es ts rvs Hetype Hbase Hlf.
   - destruct vs => //.
     inversion Hlf; subst; simpl in *.
     apply e_composition_typing in Hetype
         as [? [t0s [ts' [t1s' [Ht0s [Hts'' [Hetypervs Hetype]]]]]]].
     apply_cat0_inv Ht0s; simpl in *; subst.
     by exists t1s', C.
-  - inversion Hlf as [ | k vs0 n es'0 lh'0 es''0 es0 LI Hconst Hlf0]; subst; clear Hlf.
+  - subst. simpl in *.
+    rewrite - cat1s in Hetype.
+    repeat rewrite catA in Hlf.
     apply e_composition_typing in Hetype
-        as [? [t0s [ts' [t1s' [Ht0s [Hts'' [Hetypevs Hetype]]]]]]].
+        as [? [t0s [ts' [t1s' [Ht0s [-> [Hetypevs Hetype]]]]]]].
     apply_cat0_inv Ht0s; subst.
     apply e_composition_typing in Hetype
-        as [? [t0s' [ts'' [t1s'' [Ht0s [Hts'' [Hetypervs Hetype]]]]]]].
-    (* XXX misleading naming *)
+        as [? [t0s' [ts'' [t1s'' [-> [-> [Hetypervs Hetype]]]]]]].
     apply Label_typing in Hetypervs
         as [? [ts2' [-> [Hetypees' [HetypeLI Hlen]]]]].
     by eapply IH in HetypeLI; eauto.
@@ -2145,13 +2102,13 @@ Proof.
   repeat rewrite length_is_size; by lias.
 Qed.
 
-Lemma lfilled_return_empty_vs_base : forall lh s C ln lf es t1s t2s i rvs,
+Lemma lfilled_return_empty_vs_base : forall i (lh: lholed i) s C ln lf es t1s t2s rvs,
   e_typing s C [:: AI_local ln lf es] (Tf t1s t2s) ->
   empty_vs_base lh ->
-  lfilledInd i lh (vs_to_es rvs ++ [:: AI_basic BI_return]) es ->
+  lfill lh (vs_to_es rvs ++ [:: AI_basic BI_return]) = es ->
   length rvs >= ln.
 Proof.
-  move => lh s C ln lf es t1s t2s i rvs Hetype Hbase Hlf.
+  move => i lh s C ln lf es t1s t2s rvs Hetype Hbase Hlf.
   apply Local_typing in Hetype as [ts' [-> [Hstype Hlen']]].
   inversion Hstype as [s0 lf0 es' ret'0 ts'0 C'' C' Hftype HeqC'' Hetype _].
   subst s0 ret'0 lf0 ts'0 es' C''.
@@ -2161,8 +2118,8 @@ Qed.
 
 (* return has not returned enough values *)
 Lemma local_return_error : forall s f ln lf es rvs ves,
-  (exists i lh,
-    lfilledInd i lh (vs_to_es rvs ++ [:: AI_basic BI_return]) es /\
+  (exists i (lh: lholed i),
+    lfill lh (vs_to_es rvs ++ [:: AI_basic BI_return]) = es /\
     empty_vs_base lh) ->
   (ln <= length rvs) = false ->
   ~ fragment_typeable s f ves [:: AI_local ln lf es].
@@ -2181,7 +2138,7 @@ Lemma reduce_local_rec : forall (hs hs' : host_state) s s' f f' es es' ves ln lf
     hs' s' f (vs_to_es ves ++ [:: AI_local ln f' es']).
 Proof.
   intros hs hs' s s' f f' es es' ves ln lf IH.
-  eapply r_label with (k := 0) (lh := LH_base (vs_to_es ves) [::]);
+  eapply r_label with (k := 0) (lh := LH_base (rev ves) [::]);
     try by solve_lfilled.
   by apply r_local.
 Qed.
@@ -2944,7 +2901,7 @@ Definition terminal_form (es: seq administrative_instruction) :=
   const_list es \/ es = [::AI_trap].
 
 Definition not_lf_return (es: seq administrative_instruction) (n: nat) :=
-  forall lh, ~ lfilled n lh [::AI_basic BI_return] es.
+  forall (lh: lholed n), lfill lh [::AI_basic BI_return] <> es.
 
 (* XXX do not separate vcs and es? *)
 Lemma t_progress_e_interpreter : forall s C C' f vcs es t1s t2s lab ret (hs : host_state),
@@ -2953,7 +2910,7 @@ Lemma t_progress_e_interpreter : forall s C C' f vcs es t1s t2s lab ret (hs : ho
     inst_typing s f.(f_inst) C' ->
     map typeof vcs = t1s ->
     store_typing s ->
-    (forall n lh k, lfilled n lh [::AI_basic (BI_br k)] es -> k < n) ->
+    (forall n (lh: lholed n) k, lfill lh [::AI_basic (BI_br k)] = es -> k < n) ->
     (forall n, not_lf_return es n) ->
     terminal_form (v_to_e_list vcs ++ es) \/
     exists s' f' es' hs', reduce hs s f (v_to_e_list vcs ++ es) hs' s' f' es'.
@@ -2977,16 +2934,16 @@ Proof.
   - (* RS'_break *)
     exfalso.
     destruct Hbr as [i [j [lh [Heqj [HLF Hbase]]]]].
-    apply lfilled_collapse_empty_vs_base in HLF as [lh' HLF'] => //.
-    move/lfilledP in HLF'.
-    apply HLFbr in HLF'.
-    by lias.
+    unfold vs_to_es in HLF.
+    erewrite lfill_push_base_vs in HLF => //.
+    eapply lfill_drop_vs in HLF => //; last by apply v_to_e_is_const_list.
+    by apply HLFbr in HLF; lias.
   - (* RS'_return *)
     exfalso.
     destruct Hret as [i [lh [HLF Hbase]]].
-    apply lfilled_collapse_empty_vs_base in HLF as [lh' HLF'] => //.
-    move/lfilledP in HLF'.
-    by apply (HLFret i lh').
+    erewrite lfill_push_base_vs in HLF => //.
+    eapply lfill_drop_vs in HLF => //; last by apply v_to_e_is_const_list.
+    by apply HLFret in HLF; lias.
   - right. exists s', f', es', hs' => //.
 Qed.
 
